Generalize thread simulation

src/gsim/gCompatibility.v
@@ -50,13 +50,13 @@ Definition _sim_itree
            R_src R_tgt
            (sim_ret:SIM_VAL R_src R_tgt)
            (itr_src: itree MemE.t R_src) (itr_tgt: itree MemE.t R_tgt): Prop :=
-  forall lc_src lc_tgt sc0_src sc0_tgt mem0_src mem0_tgt w1
+  forall b lc_src lc_tgt sc0_src sc0_tgt mem0_src mem0_tgt w1
          (LOCAL: sim_local w1 lc_src lc_tgt)
          (WORLD: world_le w0 w1),
     sim_thread
       (lang R_src) (lang R_tgt)
       (sim_terminal sim_ret)
-      w1
+      b w1
       itr_src lc_src sc0_src mem0_src
       itr_tgt lc_tgt sc0_tgt mem0_tgt.
 
@@ -72,14 +72,14 @@ Definition _sim_ktree
     _sim_itree sim_thread w sim_ret1 (ktr_src r_src) (ktr_tgt r_tgt).
 
 Lemma _sim_itree_mon
-      s1 s2 (S: s1 <12= s2):
+      s1 s2 (S: s1 <13= s2):
   @_sim_itree s1 <6= @_sim_itree s2.
 Proof.
   ii. apply S. apply PR; auto.
 Qed.
 
 Lemma _sim_ktree_mon
-      s1 s2 (S: s1 <12= s2):
+      s1 s2 (S: s1 <13= s2):
   @_sim_ktree s1 <8= @_sim_ktree s2.
 Proof.
   ii. apply S. eapply PR; eauto.
@@ -265,7 +265,7 @@ Global Hint Resolve cpn11_wcompat: paco.
 
 Inductive ctx (sim_thread:SIM_THREAD world): SIM_THREAD world :=
 | ctx_ret
-    R_src R_tgt w0
+    R_src R_tgt b w0
     (sim_ret:SIM_VAL R_src R_tgt)
     sc0_src mem0_src
     sc0_tgt mem0_tgt
@@ -275,27 +275,27 @@ Inductive ctx (sim_thread:SIM_THREAD world): SIM_THREAD world :=
     @ctx sim_thread
          (lang R_src) (lang R_tgt)
          (sim_terminal sim_ret)
-         w0
+         b w0
          (Ret r_src) lc_src sc0_src mem0_src
          (Ret r_tgt) lc_tgt sc0_tgt mem0_tgt
 | ctx_bind
-    R_src0 R_tgt0 R_src1 R_tgt1 w0
+    R_src0 R_tgt0 R_src1 R_tgt1 b w0
     (sim_ret1:SIM_VAL R_src0 R_tgt0) (sim_ret2:SIM_VAL R_src1 R_tgt1)
     itr0 k0 lc_src sc0_src mem0_src
     itr1 k1 lc_tgt sc0_tgt mem0_tgt
     (SIM1: sim_thread (lang R_src0) (lang R_tgt0) (sim_terminal sim_ret1)
-                      w0
+                      b w0
                       itr0 lc_src sc0_src mem0_src
                       itr1 lc_tgt sc0_tgt mem0_tgt)
     (SIM2: _sim_ktree sim_thread sim_ret1 k0 k1 sim_ret2):
     @ctx sim_thread
          (lang R_src1) (lang R_tgt1)
          (sim_terminal sim_ret2)
-         w0
+         b w0
          (itr0 >>= k0) lc_src sc0_src mem0_src
          (itr1 >>= k1) lc_tgt sc0_tgt mem0_tgt
 | ctx_tau_iter
-    I_src I_tgt R_src R_tgt w0
+    I_src I_tgt R_src R_tgt b w0
     (sim_ret0: SIM_VAL I_src I_tgt) (sim_ret1: SIM_VAL R_src R_tgt)
     sc0_src mem0_src
     sc0_tgt mem0_tgt
@@ -310,12 +310,12 @@ Inductive ctx (sim_thread:SIM_THREAD world): SIM_THREAD world :=
     @ctx sim_thread
          (lang R_src) (lang R_tgt)
          (sim_terminal sim_ret1)
-         w0
+         b w0
          (tau;;(ITree.iter body_src i_src)) lc_src sc0_src mem0_src
          (tau;;(ITree.iter body_tgt i_tgt)) lc_tgt sc0_tgt mem0_tgt
 .
 
-Lemma ctx_mon: monotone12 ctx.
+Lemma ctx_mon: monotone13 ctx.
 Proof.
   ii. destruct IN.
   - econs 1; eauto.
@@ -339,25 +339,27 @@ Qed.
 
 Definition _sim_thread := @_sim_thread world world_le sim_memory sim_timemap sim_local.
 
-Lemma _sim_thread_mon: monotone12 _sim_thread.
+Lemma _sim_thread_mon: monotone13 _sim_thread.
 Proof.
   eapply _sim_thread_mon.
 Qed.
 
 Lemma ctx_compat:
-  ctx <13= gupaco12 _sim_thread (cpn12 _sim_thread).
+  ctx <14= gupaco13 _sim_thread (cpn13 _sim_thread).
 Proof.
-  assert (MON: monotone12 _sim_thread).
+  assert (MON: monotone13 _sim_thread).
   (* paco tactics do not work well without this *)
   { eapply _sim_thread_mon; eauto. }
-  eapply wrespect12_uclo; auto.
+  eapply wrespect13_uclo; auto.
   econs; auto. i. destruct PR.
   - (* ret *)
     ii.
     splits; s; ii.
     { right. inv TERMINAL_TGT. ss. esplits; eauto; ss.
       - econs; eauto.
-      - eapply sim_local_world_mon; eauto.
+      - eapply sim_future_memory_sc_future in FUTURE; eauto.
+        2:{ typeclasses eauto. (* why? *) }
+        des. eapply sim_local_world_mon; eauto.
       - econs; eauto.
       - refl.
     }
@@ -365,7 +367,9 @@ Proof.
     inv STEP_TGT; try by inv STEP; inv STATE.
     inv STEP; ss.
     exploit sim_local_promise; try apply MEMORY; eauto.
-    { eapply sim_local_world_mon; eauto. }
+    { eapply sim_future_memory_sc_future in FUTURE; eauto.
+      2:{ typeclasses eauto. (* why? *) }
+      des. eapply sim_local_world_mon; eauto. }
     i. des.
     right. esplits; try apply MEM2.
     + ss.
@@ -373,7 +377,7 @@ Proof.
     + econs 2. econs 1. econs; eauto.
     + eauto.
     + eapply sim_timemap_world_mon; eauto.
-    + eapply rclo12_clo_base. eapply ctx_ret; auto.
+    + eapply rclo13_clo_base. eapply ctx_ret; auto.
     + auto.
   - (* bind *)
     ii. ss. eapply GF in SIM1.
@@ -399,8 +403,11 @@ Proof.
         { eapply f_equal with (f:=observe) in TGT. ss. clarify. }
         subst.
         exploit SIM2; eauto. i. eapply GF in x0.
-        exploit x0; try apply SC0; eauto using Memory.future_future_weak.
-        { refl. }
+        exploit x0; try apply SC0; eauto.
+        { instantiate (5:=b1). red. destruct b1.
+          { splits; auto. }
+          { splits; try refl. }
+        }
         i. ss. des. exploit TERMINAL0; try by econs.
         { econs. eauto. }
         i. des.
@@ -449,8 +456,11 @@ Proof.
         { eapply f_equal with (f:=observe) in TGT. ss. clarify. }
         subst.
         exploit SIM2; eauto. i. eapply GF in x.
-        exploit x; try apply SC0; eauto using Memory.future_future_weak.
-        { refl. }
+        exploit x; try apply SC0; eauto.
+        { instantiate (5:=b1). red. destruct b1.
+          { splits; auto. }
+          { splits; try refl. }
+        }
         i. ss. des.
         exploit STEP0; eauto. i. des.
         { left.
@@ -461,7 +471,7 @@ Proof.
           etrans; eauto. rewrite bind_ret_l. eauto. }
         { right.
           esplits; cycle 2; eauto.
-          - eapply rclo12_base. auto.
+          - eapply rclo13_base. auto.
           - etrans; eauto.
           - eapply rtc_internal_step_bind in STEPS.
             etrans; [apply STEPS|eauto].
@@ -479,7 +489,7 @@ Proof.
         esplits; [|M|M| | | | |]; Mskip eauto.
         { eapply rtc_internal_step_bind. eauto. }
         { eapply opt_step_bind. eauto. }
-        { eapply rclo12_clo_base. eapply ctx_bind; eauto.
+        { eapply rclo13_clo_base. eapply ctx_bind; eauto.
           eapply _sim_ktree_mon; cycle 1; eauto.
         }
     + left. exploit STEP.
@@ -498,13 +508,15 @@ Proof.
     + (* promise *)
       inv STEP; ss.
       exploit sim_local_promise; try apply MEMORY; eauto.
-      { eapply sim_local_world_mon; eauto. }
+      { eapply sim_future_memory_sc_future in FUTURE; eauto.
+        2:{ typeclasses eauto. (* why? *) }
+        des. eapply sim_local_world_mon; eauto. }
       i. des.
       esplits; try apply MEM2; eauto; ss.
       { econs 2. econs 1. econs; eauto. }
       { eauto. }
       { eapply sim_timemap_world_mon; eauto. }
-      { eapply rclo12_clo_base. eapply ctx_tau_iter; eauto.
+      { eapply rclo13_clo_base. eapply ctx_tau_iter; eauto.
         eapply _sim_ktree_mon; cycle 1; eauto.
       }
     + (* tau *)
@@ -512,14 +524,16 @@ Proof.
       esplits; try apply MEMORY; eauto; ss.
       { econs 2. econs 2. econs; [|econs 1]; eauto. econs; eauto. }
       { rewrite unfold_iter_eq. rewrite unfold_iter_eq.
-        eapply rclo12_clo. eapply ctx_bind; eauto.
-        { eapply rclo12_base. eapply LE. eapply SIM; eauto.
+        eapply rclo13_clo. eapply ctx_bind; eauto.
+        { eapply sim_future_memory_sc_future in FUTURE; eauto.
+          2:{ typeclasses eauto. (* why? *) }
+          des. eapply rclo13_base. eapply LE. eapply SIM; eauto.
           eapply sim_local_world_mon; eauto.
         }
-        ii. eapply rclo12_clo. inv RET.
+        ii. eapply rclo13_clo. inv RET.
         { eapply ctx_tau_iter; eauto.
           eapply _sim_ktree_mon; cycle 1; eauto.
-          i. eapply rclo12_base. eauto. }
+          i. eapply rclo13_base. eauto. }
         { eapply ctx_ret; eauto. }
       }
       { refl. }
@@ -528,7 +542,7 @@ Qed.
 
 Inductive iter_ctx (sim_thread:SIM_THREAD world): SIM_THREAD world :=
 | ctx_iter
-    I_src I_tgt R_src R_tgt w0
+    I_src I_tgt R_src R_tgt b w0
     (sim_ret0: SIM_VAL I_src I_tgt) (sim_ret1: SIM_VAL R_src R_tgt)
     sc0_src mem0_src
     sc0_tgt mem0_tgt
@@ -543,12 +557,12 @@ Inductive iter_ctx (sim_thread:SIM_THREAD world): SIM_THREAD world :=
     @iter_ctx sim_thread
               (lang R_src) (lang R_tgt)
               (sim_terminal sim_ret1)
-              w0
+              b w0
               (ITree.iter body_src i_src) lc_src sc0_src mem0_src
               (ITree.iter body_tgt i_tgt) lc_tgt sc0_tgt mem0_tgt
 .
 
-Lemma iter_ctx_mon: monotone12 iter_ctx.
+Lemma iter_ctx_mon: monotone13 iter_ctx.
 Proof.
   ii. destruct IN.
   econs; eauto. ii. eapply LE. eapply SIM; eauto.
@@ -556,25 +570,25 @@ Qed.
 Hint Resolve iter_ctx_mon.
 
 Lemma iter_ctx_compat:
-  iter_ctx <13= gupaco12 _sim_thread (cpn12 _sim_thread).
+  iter_ctx <14= gupaco13 _sim_thread (cpn13 _sim_thread).
 Proof.
-  assert (MON: monotone12 _sim_thread).
+  assert (MON: monotone13 _sim_thread).
   (* paco tactics do not work well without this *)
   { eapply _sim_thread_mon; eauto. }
-  eapply grespect12_uclo; auto.
+  eapply grespect13_uclo; auto.
   econs; auto. i. destruct PR.
-  eapply rclo12_clo_base. eapply cpn12_gupaco; [eauto with paco|].
+  eapply rclo13_clo_base. eapply cpn13_gupaco; [eauto with paco|].
   rewrite unfold_iter_eq. rewrite unfold_iter_eq.
   guclo ctx_compat. eapply ctx_bind.
   { gbase. eapply _sim_thread_mon.
     { eapply GF. eapply (@SIM i_src i_tgt); eauto. refl. }
-    { i. eapply rclo12_base. eauto. }
+    { i. eapply rclo13_base. eauto. }
   }
   { ii. inv RET.
     { guclo ctx_compat. eapply ctx_tau_iter; eauto.
       eapply _sim_ktree_mon; cycle 1; eauto.
       i. gbase. eapply _sim_thread_mon; eauto.
-      i. eapply rclo12_base. eauto.
+      i. eapply rclo13_base. eauto.
     }
     { guclo ctx_compat. eapply ctx_ret; eauto. }
   }
@@ -583,25 +597,19 @@ Qed.
 Definition sim_itree := @_sim_itree (sim_thread world_le sim_memory sim_timemap sim_local).
 Definition sim_ktree := @_sim_ktree (sim_thread world_le sim_memory sim_timemap sim_local).
 
-Lemma sim_itree_mon R_src R_tgt w0 w1
+Lemma sim_itree_mon R_src R_tgt w0
       sim_ret0 sim_ret1
       itr_src itr_tgt
       (SIM01: sim_ret0 <2= sim_ret1)
-      (SIM: @sim_itree w0 R_src R_tgt sim_ret0 itr_src itr_tgt)
-      (WORLD: world_le w0 w1):
-  sim_itree w1 sim_ret1 itr_src itr_tgt.
+      (SIM: @sim_itree w0 R_src R_tgt sim_ret0 itr_src itr_tgt):
+  sim_itree w0 sim_ret1 itr_src itr_tgt.
 Proof.
-  cut (sim_itree w0 sim_ret1 itr_src itr_tgt).
-  { ii. eapply sim_thread_future; try refl.
-    { eapply world_le_PreOrder. }
-    { eapply H; eauto. etrans; eauto. }
-  }
   ii. eapply sim_thread_mon; [|eauto].
   i. inv PR. econs; eauto.
 Qed.
 
 Hint Resolve _sim_thread_mon: paco.
-Hint Resolve cpn12_wcompat: paco.
+Hint Resolve cpn13_wcompat: paco.
 
 Lemma sim_itree_ret R_src R_tgt (sim_ret: SIM_VAL R_src R_tgt)
       r_src r_tgt
