src/gsim/gSimMemory.v
@@ -36,7 +36,7 @@ Definition world: Type. Admitted.
 Definition world_le: world -> world -> Prop. Admitted.
 Instance world_le_PreOrder: PreOrder world_le. Admitted.
 
-Definition sim_memory: forall (w: world) (mem_src mem_tgt:Memory.t), Prop. Admitted.
+Definition sim_memory: forall (b: bool) (w: world) (mem_src mem_tgt:Memory.t), Prop. Admitted.
 Definition sim_timemap: forall (w: world) (sc_src sc_tgt: TimeMap.t), Prop. Admitted.
 Definition sim_local: forall (w: world) (lc_src lc_tgt:Local.t), Prop. Admitted.
 
@@ -60,7 +60,7 @@ Lemma sim_memory_cap: forall
     mem1_src mem2_src
     mem1_tgt mem2_tgt
     sc1_src sc1_tgt
-    (MEM1: sim_memory w1 mem1_src mem1_tgt)
+    (MEM1: sim_memory false w1 mem1_src mem1_tgt)
     (CAP_SRC: Memory.cap mem1_src mem2_src)
     (CAP_TGT: Memory.cap mem1_tgt mem2_tgt)
     (MEM1_SRC: Memory.closed mem1_src)
@@ -68,21 +68,21 @@ Lemma sim_memory_cap: forall
     (CLOSED_SRC: Memory.closed_timemap sc1_src mem1_src)
     (CLOSED_TGT: Memory.closed_timemap sc1_tgt mem1_tgt),
     exists w2,
-      (<<MEM2: sim_memory w2 mem2_src mem2_tgt>>) /\
+      (<<MEM2: sim_memory true w2 mem2_src mem2_tgt>>) /\
       (<<TIMEMAP: sim_timemap w2 sc1_src sc1_tgt>>) /\
       (<<WORLD: world_le w1 w2>>)
 .
 Admitted.
 
 Lemma sim_local_promise
-      w0
+      b w0
       lc1_src mem1_src
       lc1_tgt mem1_tgt
       lc2_tgt mem2_tgt
       loc from to msg_tgt kind_tgt
       (STEP_TGT: Local.promise_step lc1_tgt mem1_tgt loc from to msg_tgt lc2_tgt mem2_tgt kind_tgt)
       (LOCAL1: sim_local w0 lc1_src lc1_tgt)
-      (MEM1: sim_memory w0 mem1_src mem1_tgt)
+      (MEM1: sim_memory b w0 mem1_src mem1_tgt)
       (WF1_SRC: Local.wf lc1_src mem1_src)
       (WF1_TGT: Local.wf lc1_tgt mem1_tgt)
       (MEM1_SRC: Memory.closed mem1_src)
@@ -90,6 +90,6 @@ Lemma sim_local_promise
   exists lc2_src mem2_src msg_src kind_src w1,
     (<<STEP_SRC: Local.promise_step lc1_src mem1_src loc from to msg_src lc2_src mem2_src kind_src>>) /\
     (<<LOCAL2: sim_local w1 lc2_src lc2_tgt>>) /\
-    (<<MEM2: sim_memory w1 mem2_src mem2_tgt>>) /\
+    (<<MEM2: sim_memory b w1 mem2_src mem2_tgt>>) /\
     (<<WORLD: world_le w0 w1>>).
 Admitted.
