src/gsim/gSimulation.v
@@ -47,7 +47,7 @@ Section WORLD.
 Variable world: Type.
 Variable world_le: world -> world -> Prop.
 
-Hypothesis world_le_PreOrder: PreOrder world_le.
+Context `{world_le_PreOrder: @PreOrder _ world_le}.
 
 Variable sim_memory: forall (b: bool) (w: world) (mem_src mem_tgt:Memory.t), Prop.
 Variable sim_timemap: forall (w: world) (sc_src sc_tgt: TimeMap.t), Prop.
@@ -145,7 +145,7 @@ Section SimulationThread.
       (<<SCSRC: sc1_src = sc0_src>>) /\
       (<<SCTGT: sc1_tgt = sc0_tgt>>) /\
       (<<WORLD: w1 = w0>>)
-    end.      
+    end.
 
   Lemma sim_future_memory_sc_future
         (b0 b1: bool)
@@ -174,7 +174,7 @@ Section SimulationThread.
       { auto. }
     - splits; auto.
   Qed.
-  
+
   Definition _sim_thread
              (sim_thread: SIM_THREAD)
              (lang_src lang_tgt:language)
@@ -201,7 +201,7 @@ Section SimulationThread.
            (FUTURE: sim_memory_future
                       b0 b1
                       lc1_src.(Local.promises) lc1_tgt.(Local.promises)
-                      mem0_src mem1_src mem0_tgt mem1_tgt                      
+                      mem0_src mem1_src mem0_tgt mem1_tgt
                       sc0_src sc1_src sc0_tgt sc1_tgt
                       w0 w1),
       (<<TERMINAL:
@@ -260,12 +260,30 @@ Section SimulationThread.
 End SimulationThread.
 Hint Resolve _sim_thread_mon: paco.
 
+Definition sim_thread_past lang_src lang_tgt sim_terminal (b: bool) w st_src lc_src sc_src mem_src st_tgt lc_tgt sc_tgt mem_tgt :=
+  if b
+  then sim_thread sim_terminal true w st_src lc_src sc_src mem_src st_tgt lc_tgt sc_tgt mem_tgt
+  else exists w' sc_src' mem_src' sc_tgt' mem_tgt',
+      (<<SIM: @sim_thread lang_src lang_tgt sim_terminal false w' st_src lc_src sc_src' mem_src' st_tgt lc_tgt sc_tgt' mem_tgt'>>) /\
+      (<<SC_FUTURE_SRC: TimeMap.le sc_src' sc_src>>) /\
+      (<<SC_FUTURE_TGT: TimeMap.le sc_tgt' sc_tgt>>) /\
+      (<<MEM_FUTURE_SRC: Memory.future_weak mem_src' mem_src>>) /\
+      (<<MEM_FUTURE_TGT: Memory.future_weak mem_tgt' mem_tgt>>) /\
+      (<<WORLD: world_le w' w>>)
+.
+Arguments sim_thread_past: simpl never.
+
+Lemma sim_thread_sim_thread_past:
+  sim_thread <13= sim_thread_past.
+Proof.
+  ii. red. destruct x3; auto. esplits; eauto; try refl.
+Qed.
 
 Lemma sim_thread_step
       lang_src lang_tgt
       sim_terminal
       pf_tgt e_tgt
-      b1 w1
+      b w1
       st1_src lc1_src sc1_src mem1_src
       st1_tgt lc1_tgt sc1_tgt mem1_tgt
       st3_tgt lc3_tgt sc3_tgt mem3_tgt
@@ -273,7 +291,7 @@ Lemma sim_thread_step
                           (Thread.mk _ st1_tgt lc1_tgt sc1_tgt mem1_tgt)
                           (Thread.mk _ st3_tgt lc3_tgt sc3_tgt mem3_tgt))
       (SC: sim_timemap w1 sc1_src sc1_tgt)
-      (MEMORY: sim_memory b1 w1 mem1_src mem1_tgt)
+      (MEMORY: sim_memory b w1 mem1_src mem1_tgt)
       (WF_SRC: Local.wf lc1_src mem1_src)
       (WF_TGT: Local.wf lc1_tgt mem1_tgt)
       (SC_SRC: Memory.closed_timemap sc1_src mem1_src)
@@ -281,7 +299,7 @@ Lemma sim_thread_step
       (MEM_SRC: Memory.closed mem1_src)
       (MEM_TGT: Memory.closed mem1_tgt)
       (CONS_TGT: Local.promise_consistent lc3_tgt)
-      (SIM: sim_thread sim_terminal b1 w1 st1_src lc1_src sc1_src mem1_src st1_tgt lc1_tgt sc1_tgt mem1_tgt):
+      (SIM: sim_thread_past sim_terminal b w1 st1_src lc1_src sc1_src mem1_src st1_tgt lc1_tgt sc1_tgt mem1_tgt):
   (<<FAILURE: Thread.steps_failure (Thread.mk lang_src st1_src lc1_src sc1_src mem1_src)>>) \/
   exists e_src st2_src lc2_src sc2_src mem2_src st3_src lc3_src sc3_src mem3_src w3,
     (<<FAILURE: ThreadEvent.get_machine_event e_tgt <> MachineEvent.failure>>) /\
@@ -293,33 +311,43 @@ Lemma sim_thread_step
                             (Thread.mk _ st3_src lc3_src sc3_src mem3_src)>>) /\
     (<<EVENT: ThreadEvent.get_machine_event e_src = ThreadEvent.get_machine_event e_tgt>>) /\
     (<<SC: sim_timemap w3 sc3_src sc3_tgt>>) /\
-    (<<MEMORY: sim_memory b1 w3 mem3_src mem3_tgt>>) /\
+    (<<MEMORY: sim_memory b w3 mem3_src mem3_tgt>>) /\
     (<<WF_SRC: Local.wf lc3_src mem3_src>>) /\
     (<<WF_TGT: Local.wf lc3_tgt mem3_tgt>>) /\
     (<<SC_SRC: Memory.closed_timemap sc3_src mem3_src>>) /\
     (<<SC_TGT: Memory.closed_timemap sc3_tgt mem3_tgt>>) /\
     (<<MEM_SRC: Memory.closed mem3_src>>) /\
     (<<MEM_TGT: Memory.closed mem3_tgt>>) /\
-    (<<SIM: sim_thread sim_terminal b1 w3 st3_src lc3_src sc3_src mem3_src st3_tgt lc3_tgt sc3_tgt mem3_tgt>>) /\
+    (<<SIM: sim_thread sim_terminal b w3 st3_src lc3_src sc3_src mem3_src st3_tgt lc3_tgt sc3_tgt mem3_tgt>>) /\
     (<<WORLD: world_le w1 w3>>).
 Proof.
-  hexploit step_promise_consistent; eauto. s. i.
-  punfold SIM. exploit SIM; eauto; try refl.
-  { destruct b1; ss. splits; try refl. }
-  i. des.
-  exploit Thread.step_future; eauto. s. i. des.
-  exploit STEP0; eauto. i. des; eauto.
-  inv SIM0; [|done]. right.
-  exploit Thread.rtc_tau_step_future; eauto. s. i. des.
-  exploit Thread.opt_step_future; eauto. s. i. des.
-  esplits; eauto.
+  hexploit step_promise_consistent; eauto. s. i. red in SIM. destruct b; ss.
+  { punfold SIM. exploit SIM; eauto; ss.
+    i. des.
+    exploit Thread.step_future; eauto. s. i. des.
+    exploit STEP0; eauto. i. des; eauto.
+    inv SIM0 ; [|done]. right.
+    exploit Thread.rtc_tau_step_future; eauto. s. i. des.
+    exploit Thread.opt_step_future; eauto. s. i. des.
+    esplits; eauto.
+  }
+  { des.
+    punfold SIM0. exploit SIM0; eauto; ss.
+    i. des.
+    exploit Thread.step_future; eauto. s. i. des.
+    exploit STEP0; eauto. i. des; eauto.
+    inv SIM ; [|done]. right.
+    exploit Thread.rtc_tau_step_future; eauto. s. i. des.
+    exploit Thread.opt_step_future; eauto. s. i. des.
+    esplits; eauto.
+  }
 Qed.
 
 Lemma sim_thread_opt_step
       lang_src lang_tgt
       sim_terminal
       e_tgt
-      b1 w1
+      b w1
       st1_src lc1_src sc1_src mem1_src
       st1_tgt lc1_tgt sc1_tgt mem1_tgt
       st3_tgt lc3_tgt sc3_tgt mem3_tgt
@@ -327,7 +355,7 @@ Lemma sim_thread_opt_step
                               (Thread.mk _ st1_tgt lc1_tgt sc1_tgt mem1_tgt)
                               (Thread.mk _ st3_tgt lc3_tgt sc3_tgt mem3_tgt))
       (SC: sim_timemap w1 sc1_src sc1_tgt)
-      (MEMORY: sim_memory b1 w1 mem1_src mem1_tgt)
+      (MEMORY: sim_memory b w1 mem1_src mem1_tgt)
       (WF_SRC: Local.wf lc1_src mem1_src)
       (WF_TGT: Local.wf lc1_tgt mem1_tgt)
       (SC_SRC: Memory.closed_timemap sc1_src mem1_src)
@@ -335,7 +363,7 @@ Lemma sim_thread_opt_step
       (MEM_SRC: Memory.closed mem1_src)
       (MEM_TGT: Memory.closed mem1_tgt)
       (CONS_TGT: Local.promise_consistent lc3_tgt)
-      (SIM: sim_thread sim_terminal b1 w1 st1_src lc1_src sc1_src mem1_src st1_tgt lc1_tgt sc1_tgt mem1_tgt):
+      (SIM: sim_thread_past sim_terminal b w1 st1_src lc1_src sc1_src mem1_src st1_tgt lc1_tgt sc1_tgt mem1_tgt):
   (<<FAILURE: Thread.steps_failure (Thread.mk lang_src st1_src lc1_src sc1_src mem1_src)>>) \/
   exists e_src st2_src lc2_src sc2_src mem2_src st3_src lc3_src sc3_src mem3_src w3,
     (<<FAILURE: ThreadEvent.get_machine_event e_tgt <> MachineEvent.failure>>) /\
@@ -347,14 +375,14 @@ Lemma sim_thread_opt_step
                              (Thread.mk _ st3_src lc3_src sc3_src mem3_src)>>) /\
     (<<EVENT: ThreadEvent.get_machine_event e_src = ThreadEvent.get_machine_event e_tgt>>) /\
     (<<SC: sim_timemap w3 sc3_src sc3_tgt>>) /\
-    (<<MEMORY: sim_memory b1 w3 mem3_src mem3_tgt>>) /\
+    (<<MEMORY: sim_memory b w3 mem3_src mem3_tgt>>) /\
     (<<WF_SRC: Local.wf lc3_src mem3_src>>) /\
     (<<WF_TGT: Local.wf lc3_tgt mem3_tgt>>) /\
     (<<SC_SRC: Memory.closed_timemap sc3_src mem3_src>>) /\
     (<<SC_TGT: Memory.closed_timemap sc3_tgt mem3_tgt>>) /\
     (<<MEM_SRC: Memory.closed mem3_src>>) /\
     (<<MEM_TGT: Memory.closed mem3_tgt>>) /\
-    (<<SIM: sim_thread sim_terminal b1 w3 st3_src lc3_src sc3_src mem3_src st3_tgt lc3_tgt sc3_tgt mem3_tgt>>) /\
+    (<<SIM: sim_thread_past sim_terminal b w3 st3_src lc3_src sc3_src mem3_src st3_tgt lc3_tgt sc3_tgt mem3_tgt>>) /\
     (<<WORLD: world_le w1 w3>>)
 .
 Proof.
@@ -362,18 +390,19 @@ Proof.
   - right. esplits; eauto; ss.
     { econs 1. }
     { refl. }
-  - eapply sim_thread_step; eauto.
+  - exploit sim_thread_step; eauto. i. des; eauto.
+    right. esplits; eauto. eapply sim_thread_sim_thread_past; eauto.
 Qed.
 
 Lemma sim_thread_rtc_step
       lang_src lang_tgt
       sim_terminal
-      b1 w1
+      b w1
       st1_src lc1_src sc1_src mem1_src
       e1_tgt e2_tgt
       (STEPS: rtc (@Thread.tau_step lang_tgt) e1_tgt e2_tgt)
       (SC: sim_timemap w1 sc1_src (Thread.sc e1_tgt))
-      (MEMORY: sim_memory b1 w1 mem1_src (Thread.memory e1_tgt))
+      (MEMORY: sim_memory b w1 mem1_src (Thread.memory e1_tgt))
       (WF_SRC: Local.wf lc1_src mem1_src)
       (WF_TGT: Local.wf (Thread.local e1_tgt) (Thread.memory e1_tgt))
       (SC_SRC: Memory.closed_timemap sc1_src mem1_src)
@@ -381,21 +410,21 @@ Lemma sim_thread_rtc_step
       (MEM_SRC: Memory.closed mem1_src)
       (MEM_TGT: Memory.closed (Thread.memory e1_tgt))
       (CONS_TGT: Local.promise_consistent (Thread.local e2_tgt))
-      (SIM: sim_thread sim_terminal b1 w1 st1_src lc1_src sc1_src mem1_src (Thread.state e1_tgt) (Thread.local e1_tgt) (Thread.sc e1_tgt) (Thread.memory e1_tgt)):
+      (SIM: sim_thread_past sim_terminal b w1 st1_src lc1_src sc1_src mem1_src (Thread.state e1_tgt) (Thread.local e1_tgt) (Thread.sc e1_tgt) (Thread.memory e1_tgt)):
   (<<FAILURE: Thread.steps_failure (Thread.mk lang_src st1_src lc1_src sc1_src mem1_src)>>) \/
   exists st2_src lc2_src sc2_src mem2_src w2,
     (<<STEPS: rtc (@Thread.tau_step lang_src)
                   (Thread.mk _ st1_src lc1_src sc1_src mem1_src)
                   (Thread.mk _ st2_src lc2_src sc2_src mem2_src)>>) /\
     (<<SC: sim_timemap w2 sc2_src (Thread.sc e2_tgt)>>) /\
-    (<<MEMORY: sim_memory b1 w2 mem2_src (Thread.memory e2_tgt)>>) /\
+    (<<MEMORY: sim_memory b w2 mem2_src (Thread.memory e2_tgt)>>) /\
     (<<WF_SRC: Local.wf lc2_src mem2_src>>) /\
     (<<WF_TGT: Local.wf (Thread.local e2_tgt) (Thread.memory e2_tgt)>>) /\
     (<<SC_SRC: Memory.closed_timemap sc2_src mem2_src>>) /\
     (<<SC_TGT: Memory.closed_timemap (Thread.sc e2_tgt) (Thread.memory e2_tgt)>>) /\
     (<<MEM_SRC: Memory.closed mem2_src>>) /\
     (<<MEM_TGT: Memory.closed (Thread.memory e2_tgt)>>) /\
-    (<<SIM: sim_thread sim_terminal b1 w2 st2_src lc2_src sc2_src mem2_src (Thread.state e2_tgt) (Thread.local e2_tgt) (Thread.sc e2_tgt) (Thread.memory e2_tgt)>>) /\
+    (<<SIM: sim_thread_past sim_terminal b w2 st2_src lc2_src sc2_src mem2_src (Thread.state e2_tgt) (Thread.local e2_tgt) (Thread.sc e2_tgt) (Thread.memory e2_tgt)>>) /\
     (<<WORLD: world_le w1 w2>>)
 .
 Proof.
@@ -407,7 +436,9 @@ Proof.
   exploit Thread.step_future; eauto. s. i. des.
   hexploit rtc_tau_step_promise_consistent; eauto. s. i.
   exploit sim_thread_step; eauto. i. des; eauto.
-  exploit IHSTEPS; eauto. i. des.
+  exploit IHSTEPS; eauto.
+  { eapply sim_thread_sim_thread_past. eauto. }
+  i. des.
   - left. inv FAILURE0. des.
     unfold Thread.steps_failure. esplits; [|eauto|eauto].
     etrans; eauto. etrans; eauto. inv STEP0; eauto.
@@ -427,13 +458,13 @@ Lemma sim_thread_plus_step
       lang_src lang_tgt
       sim_terminal
       pf_tgt e_tgt
-      b1 w1
+      b w1
       st1_src lc1_src sc1_src mem1_src
       e1_tgt e2_tgt e3_tgt
       (STEPS: rtc (@Thread.tau_step lang_tgt) e1_tgt e2_tgt)
       (STEP: @Thread.step lang_tgt pf_tgt e_tgt e2_tgt e3_tgt)
       (SC: sim_timemap w1 sc1_src (Thread.sc e1_tgt))
-      (MEMORY: sim_memory b1 w1 mem1_src (Thread.memory e1_tgt))
+      (MEMORY: sim_memory b w1 mem1_src (Thread.memory e1_tgt))
       (WF_SRC: Local.wf lc1_src mem1_src)
       (WF_TGT: Local.wf (Thread.local e1_tgt) (Thread.memory e1_tgt))
       (SC_SRC: Memory.closed_timemap sc1_src mem1_src)
@@ -441,7 +472,7 @@ Lemma sim_thread_plus_step
       (MEM_SRC: Memory.closed mem1_src)
       (MEM_TGT: Memory.closed (Thread.memory e1_tgt))
       (CONS_TGT: Local.promise_consistent (Thread.local e3_tgt))
-      (SIM: sim_thread sim_terminal b1 w1 st1_src lc1_src sc1_src mem1_src (Thread.state e1_tgt) (Thread.local e1_tgt) (Thread.sc e1_tgt) (Thread.memory e1_tgt)):
+      (SIM: sim_thread_past sim_terminal b w1 st1_src lc1_src sc1_src mem1_src (Thread.state e1_tgt) (Thread.local e1_tgt) (Thread.sc e1_tgt) (Thread.memory e1_tgt)):
   (<<FAILURE: Thread.steps_failure (Thread.mk lang_src st1_src lc1_src sc1_src mem1_src)>>) \/
   exists e_src st2_src lc2_src sc2_src mem2_src st3_src lc3_src sc3_src mem3_src w3,
     (<<FAILURE: ThreadEvent.get_machine_event e_tgt <> MachineEvent.failure>>) /\
@@ -453,14 +484,14 @@ Lemma sim_thread_plus_step
                             (Thread.mk _ st3_src lc3_src sc3_src mem3_src)>>) /\
     (<<EVENT: ThreadEvent.get_machine_event e_src = ThreadEvent.get_machine_event e_tgt>>) /\
     (<<SC: sim_timemap w3 sc3_src (Thread.sc e3_tgt)>>) /\
-    (<<MEMORY: sim_memory b1 w3 mem3_src (Thread.memory e3_tgt)>>) /\
+    (<<MEMORY: sim_memory b w3 mem3_src (Thread.memory e3_tgt)>>) /\
     (<<WF_SRC: Local.wf lc3_src mem3_src>>) /\
     (<<WF_TGT: Local.wf (Thread.local e3_tgt) (Thread.memory e3_tgt)>>) /\
     (<<SC_SRC: Memory.closed_timemap sc3_src mem3_src>>) /\
     (<<SC_TGT: Memory.closed_timemap (Thread.sc e3_tgt) (Thread.memory e3_tgt)>>) /\
     (<<MEM_SRC: Memory.closed mem3_src>>) /\
     (<<MEM_TGT: Memory.closed (Thread.memory e3_tgt)>>) /\
-    (<<SIM: sim_thread sim_terminal b1 w3 st3_src lc3_src sc3_src mem3_src (Thread.state e3_tgt) (Thread.local e3_tgt) (Thread.sc e3_tgt) (Thread.memory e3_tgt)>>) /\
+    (<<SIM: sim_thread sim_terminal b w3 st3_src lc3_src sc3_src mem3_src (Thread.state e3_tgt) (Thread.local e3_tgt) (Thread.sc e3_tgt) (Thread.memory e3_tgt)>>) /\
     (<<WORLD: world_le w1 w3>>)
 .
 Proof.
@@ -499,57 +530,19 @@ Lemma sim_thread_future
       sim_terminal
       st_src lc_src sc1_src sc2_src mem1_src mem2_src w1
       st_tgt lc_tgt sc1_tgt sc2_tgt mem1_tgt mem2_tgt w2
-      (SIM: @sim_thread lang_src lang_tgt sim_terminal false w1 st_src lc_src sc1_src mem1_src st_tgt lc_tgt sc1_tgt mem1_tgt)
+      (SIM: @sim_thread_past lang_src lang_tgt sim_terminal false w1 st_src lc_src sc1_src mem1_src st_tgt lc_tgt sc1_tgt mem1_tgt)
       (SC_FUTURE_SRC: TimeMap.le sc1_src sc2_src)
       (SC_FUTURE_TGT: TimeMap.le sc1_tgt sc2_tgt)
       (MEM_FUTURE_SRC: Memory.future_weak mem1_src mem2_src)
       (MEM_FUTURE_TGT: Memory.future_weak mem1_tgt mem2_tgt)
       (WORLD: world_le w1 w2):
-  sim_thread sim_terminal false w2 st_src lc_src sc2_src mem2_src st_tgt lc_tgt sc2_tgt mem2_tgt.
+  sim_thread_past sim_terminal false w2 st_src lc_src sc2_src mem2_src st_tgt lc_tgt sc2_tgt mem2_tgt.
 Proof.
-  pfold. ii.
-  punfold SIM. exploit SIM; eauto. destruct b1; ss.
-  { des. splits; auto. etrans; eauto. }
-  { des. splits; auto. etrans; eauto. }
-Qed.  
-
-Lemma sim_thread_future
-      lang_src lang_tgt
-      sim_terminal
-      st_src lc_src sc1_src sc2_src mem1_src mem2_src w1
-      st_tgt lc_tgt sc1_tgt sc2_tgt mem1_tgt mem2_tgt w2
-      (SIM: @sim_thread lang_src lang_tgt sim_terminal false w1 st_src lc_src sc1_src mem1_src st_tgt lc_tgt sc1_tgt mem1_tgt)
-      (SC_FUTURE_SRC: TimeMap.le sc1_src sc2_src)
-      (SC_FUTURE_TGT: TimeMap.le sc1_tgt sc2_tgt)
-      (MEM_FUTURE_SRC: Memory.future_weak mem1_src mem2_src)
-      (MEM_FUTURE_TGT: Memory.future_weak mem1_tgt mem2_tgt)
-      (WORLD: world_le w1 w2):
-  sim_thread sim_terminal false w2 st_src lc_src sc1_src mem1_src st_tgt lc_tgt sc1_tgt mem1_tgt.
-Proof.
-  pfold. ii.
-  punfold SIM. exploit SIM; eauto. destruct b1; ss.
-  { des. splits; auto. etrans; eauto. }
-  { des. splits; auto. etrans; eauto. }
-Qed.  
-
-Lemma sim_thread_future
-      lang_src lang_tgt
-      sim_terminal
-      st_src lc_src sc1_src sc2_src mem1_src mem2_src w1
-      st_tgt lc_tgt sc1_tgt sc2_tgt mem1_tgt mem2_tgt w2
-      (SIM: @sim_thread lang_src lang_tgt sim_terminal false w1 st_src lc_src sc1_src mem1_src st_tgt lc_tgt sc1_tgt mem1_tgt)
-      (SC_FUTURE_SRC: TimeMap.le sc1_src sc2_src)
-      (SC_FUTURE_TGT: TimeMap.le sc1_tgt sc2_tgt)
-      (MEM_FUTURE_SRC: Memory.future_weak mem1_src mem2_src)
-      (MEM_FUTURE_TGT: Memory.future_weak mem1_tgt mem2_tgt)
-      (WORLD: world_le w1 w2):
-  sim_thread sim_terminal false w2 st_src lc_src sc2_src mem2_src st_tgt lc_tgt sc2_tgt mem2_tgt.
-Proof.
-  pfold. ii.
-  punfold SIM. exploit SIM; eauto. destruct b1; ss.
-  { des. splits; auto. etrans; eauto. }
-  { des. splits; auto. etrans; eauto. }
-Qed.  
+  red in SIM. red. des. ss. esplits; eauto.
+  { etrans; eauto. }
+  { etrans; eauto. }
+  { etrans; eauto. }
+Qed.
 
 Lemma cap_property
       mem1 mem2 lc sc
@@ -836,7 +829,7 @@ Lemma sim_thread_sim
           IdentMap.find tid ths_src = Some (existT _ lang_src st_src, lc_src) ->
           IdentMap.find tid ths_tgt = Some (existT _ lang_tgt st_tgt, lc_tgt) ->
           exists sim_terminal,
-            @sim_thread lang_src lang_tgt sim_terminal false w st_src lc_src sc0_src mem0_src st_tgt lc_tgt sc0_tgt mem0_tgt)
+            @sim_thread_past lang_src lang_tgt sim_terminal false w st_src lc_src sc0_src mem0_src st_tgt lc_tgt sc0_tgt mem0_tgt)
   :
     sim w ths_src sc0_src mem0_src ths_tgt sc0_tgt mem0_tgt.
 Proof.
@@ -860,7 +853,7 @@ Proof.
                IdentMap.find tid ths_src = Some (existT _ lang_src st_src, lc_src) ->
                IdentMap.find tid ths_tgt = Some (existT _ lang_tgt st_tgt, lc_tgt) ->
                exists sim_terminal,
-                 @sim_thread lang_src lang_tgt sim_terminal false w st_src lc_src sc0_src mem0_src st_tgt lc_tgt sc0_tgt mem0_tgt).
+                 @sim_thread_past lang_src lang_tgt sim_terminal false w st_src lc_src sc0_src mem0_src st_tgt lc_tgt sc0_tgt mem0_tgt).
     { eauto. }
     assert (TIDS_MEM: forall tid, List.In tid (IdentSet.elements tids) -> IdentSet.mem tid tids = true).
     { i. rewrite IdentSet.mem_spec.
@@ -890,10 +883,13 @@ Proof.
     exploit (IN a); eauto. i. des.
     exploit TERMINAL_TGT; eauto. i. des.
     hexploit Local.terminal_promise_consistent; eauto. i.
-    punfold x2.
-    exploit x2; try exact x; try exact x0; try exact SC; try exact SC0;
-      eauto using Memory.future_future_weak.
-    { ss. splits; eauto using Memory.future_future_weak. }
+    red in x2. des. punfold SIM0.
+    exploit SIM0; try exact x; try exact x0; try exact SC; try exact SC0; eauto.
+    { ss. splits; eauto using Memory.future_future_weak.
+      { etrans; eauto. eapply Memory.future_future_weak; eauto. }
+      { etrans; eauto. eapply Memory.future_future_weak; eauto. }
+      { etrans; eauto. }
+    }
     i. des.
     exploit TERMINAL; eauto. i. des.
     + (* failure *)
@@ -919,14 +915,14 @@ Proof.
       { rewrite IdentMap.gsspec in H0. revert H0. condtac; ss; i.
         - subst. inv NODUP. congr.
         - exploit IN; eauto. i. des.
-          esplits. eauto. eapply sim_thread_future_world; eauto; try refl. }
+          esplits. eapply sim_thread_future; eauto; try refl. }
       { inv NODUP. ss. }
       des.
       * left.
         unfold Configuration.steps_failure in *. des.
-        rewrite STEPS0 in x3. esplits; try exact x3; eauto.
+        rewrite STEPS0 in x2. esplits; try exact x2; eauto.
       * right.
-        rewrite x1 in x3. esplits; try exact x3; eauto. etrans; eauto.
+        rewrite x1 in x2. esplits; try exact x2; eauto. etrans; eauto.
 
   - (* STEP CASE *)
     i. inv STEP_TGT. destruct e2. ss.
@@ -963,7 +959,7 @@ Proof.
             * rewrite TIDS_TGT.
               rewrite Threads.tids_add. rewrite IdentSet.add_mem; ss.
               rewrite Threads.tids_o. rewrite TID. ss.
-            * i. Configuration.simplify; [eexists; eauto|].
+            * i. apply sim_thread_sim_thread_past in SIM1. Configuration.simplify; [eexists; eauto|].
               exploit Thread.rtc_tau_step_future; try exact STEPS; eauto. s. i. des.
               exploit Thread.step_future; try exact STEP; eauto. s. i. des.
               exploit Thread.rtc_tau_step_future; try exact X; eauto. s. i. des.
@@ -980,7 +976,7 @@ Proof.
             * rewrite TIDS_TGT.
               rewrite Threads.tids_add. rewrite IdentSet.add_mem; ss.
               rewrite Threads.tids_o. rewrite TID. ss.
-            * i. Configuration.simplify.
+            * i. apply sim_thread_sim_thread_past in SIM1. Configuration.simplify.
               { rewrite FIND_SRC in H. inv H. Configuration.simplify.
                 eexists; eauto. }
               { exploit Thread.rtc_tau_step_future; try exact STEPS; eauto. s. i. des.
@@ -1001,7 +997,7 @@ Proof.
           + rewrite TIDS_TGT.
             rewrite Threads.tids_add. rewrite IdentSet.add_mem; ss.
             rewrite Threads.tids_o. rewrite TID. ss.
-          + i. Configuration.simplify; [eexists; eauto|].
+          + i. apply sim_thread_sim_thread_past in SIM1. Configuration.simplify; [eexists; eauto|].
             exploit Thread.rtc_tau_step_future; try exact STEPS; eauto. s. i. des.
             exploit Thread.step_future; try exact STEP; eauto. s. i. des.
             exploit Thread.rtc_tau_step_future; try exact STEPS0; eauto. s. i. des.
